two example updated - Hu

transaction.v
@@ -94,11 +94,11 @@ Inductive action:=
 |abort_txn: action
 (*|restart_txn: action*)
 |complete_write_item: (*value -> action*)version -> action
-|unlock_write_item: version -> action
+(*|unlock_write_item: version -> action*)
 (*|invalid_write_item: value -> action*)
 |commit_txn: version -> action
 |obtain_global_tid: action.
-
+(*sp later than last lock*)
 Definition trace := list (tid * action).
 
 (*
@@ -113,6 +113,16 @@ Returns all commit actions in the trace.
 Definition trace_filter_commit tr: trace :=
     filter (fun pr => match snd pr with
                       | commit_txn _ => true
+                      | _ => false
+                      end) tr.
+
+(*
+Returns all commit actions in the trace. (for commit version update)
+*)
+Definition trace_filter_commit_complete tr: trace :=
+    filter (fun pr => match snd pr with
+                      | commit_txn _ => true
+                      | complete_write_item _ => true
                       | _ => false
                       end) tr.
 
@@ -134,6 +144,17 @@ Definition trace_commit_last t: version :=
   end.
 
 (*
+Returns the version number of the last commit/complete_write
+If there is no commit in the trace, returns 0.
+*)
+Definition trace_commit_complete_last t: version :=
+  match hd dummy (map snd (trace_filter_commit_complete t)) with 
+	| commit_txn n => n
+  | complete_write_item n => n
+	| _ => 0
+  end.
+
+(*
 Returns all lock_write_item actions in the trace.
 *)
 Definition trace_filter_lock tr: trace :=
@@ -143,11 +164,13 @@ Definition trace_filter_lock tr: trace :=
                       end) tr.
 
 (*
-Returns all unlock_write_item actions in the trace.
+All commit and abort have unlock_write_item.
+Returns all 'unlock_write_item' actions in the trace.
 *)
 Definition trace_filter_unlock tr: trace :=
     filter (fun pr => match snd pr with
-                      | unlock_write_item _ => true
+                      | commit_txn _ => true
+                      | abort_txn => true
                       | _ => false
                       end) tr.
 
@@ -162,7 +185,7 @@ Returns T if there exists lock_write_item
 *)
 Definition check_lock_or_unlock tr: Prop :=
   match 
-    length (trace_filter_lock tr) =? length (trace_filter_unlock tr)  
+    length (trace_filter_lock tr) <=? length (trace_filter_unlock tr)  
   with 
 	| true => True
 	| false => False
@@ -211,6 +234,32 @@ Function check_version (vs : list version) (v : version) : Prop :=
   | hd :: tail => if hd =? v then check_version tail v
                   else False
   end.
+(*
+Returns all start/read/write actions in the trace.
+*)
+Definition trace_filter_startreadwrite tid tr: trace :=
+    filter (fun pr => (fst pr =? tid) &&
+                      (match snd pr with
+                      | read_item _ => true
+                      | write_item _ => true
+                      | start_txn => true
+                      | _ => false
+                      end)) tr.
+
+(*
+Returns all newtid with start/read/write actions in the trace.
+*)
+Function trace_rollback (newtid: nat) (newver: version) (tr:trace): trace :=
+    match tr with 
+    | [] => []
+    | (tid, read_item _) :: tr' 
+      => [(newtid, read_item newver)] ++ trace_rollback newtid newver tr'
+    | (tid, write_item val) :: tr'
+      => [(newtid, write_item val)] ++ trace_rollback newtid newver tr'
+    | (tid, start_txn) :: tr'
+      => [(newtid, start_txn)] ++ trace_rollback newtid newver tr'
+    | _ :: tr' => trace_rollback newtid newver tr'
+  end.
 
 Inductive sto_trace : trace -> Prop :=
 
@@ -247,9 +296,6 @@ Inductive sto_trace : trace -> Prop :=
 			trace_tid_last tid t = try_commit_txn
 			/\ ~ trace_no_writes tid t
       -> check_lock_or_unlock t
-(****************************************)
-(*Note!!!!!! abort or just wait for lock*)
-(****************************************)
 			-> sto_trace t
 			-> sto_trace ((tid, lock_write_item) :: t)
 
@@ -260,10 +306,7 @@ Inductive sto_trace : trace -> Prop :=
 			-> sto_trace ((tid, validate_read_item (check_version (read_versions_tid tid t)  (trace_commit_last t) ))::t)
 
 (****************************************)
-(*Note!!!!!! *)
-(****************************************)
-
-| abort_readonly_txn_step: forall t tid,
+(*| abort_readonly_txn_step: forall t tid,
       trace_tid_last tid t = validate_read_item False (*invalid*)
       /\ trace_no_writes tid t
       -> sto_trace t
@@ -273,7 +316,13 @@ Inductive sto_trace : trace -> Prop :=
       trace_tid_last tid t = validate_read_item False (*invalid*)
       /\ ~ trace_no_writes tid t
       -> sto_trace t
-      -> sto_trace ([(tid, abort_txn); (tid, unlock_write_item (trace_commit_last t))] ++ t)
+      -> sto_trace ([(tid, abort_txn); (tid, unlock_write_item (trace_commit_last t))] ++ t)*)
+(****************************************)
+
+| abort_txn_step: forall t tid,
+      trace_tid_last tid t = validate_read_item False 
+      -> sto_trace t
+      -> sto_trace ((tid, abort_txn) :: t) (*abort will contain unlock....*)
       
 | complete_write_item_step: forall t tid,
 			trace_tid_last tid t = validate_read_item True (*valid read*)
@@ -281,13 +330,14 @@ Inductive sto_trace : trace -> Prop :=
       -> sto_trace t
       -> sto_trace ((tid, complete_write_item (S (trace_commit_last t))) :: t)
 
-| unlock_write_item_step: forall t tid ver,
+(*| unlock_write_item_step: forall t tid ver,
       trace_tid_last tid t = complete_write_item ver
 			/\ ~ trace_no_writes tid t (*locked*)
       -> sto_trace t
-      -> sto_trace ((tid, unlock_write_item ver) :: t)
+      -> sto_trace ((tid, unlock_write_item ver) :: t)*)
 
-| commit_readonly_txn_step: forall t tid,
+(****************************************)
+(*| commit_readonly_txn_step: forall t tid,
       (trace_tid_last tid t = validate_read_item True /\ trace_no_writes tid t)(*read only*)
       -> sto_trace t
       -> sto_trace ((tid, commit_txn (trace_commit_last t)) :: t)
@@ -295,115 +345,70 @@ Inductive sto_trace : trace -> Prop :=
 | commit_write_txn_step: forall t tid ver,
       trace_tid_last tid t = unlock_write_item ver(*unlock the write*)
       -> sto_trace t
-      -> sto_trace ((tid, commit_txn ver) :: t)
+      -> sto_trace ((tid, commit_txn ver) :: t).*)
+(****************************************)
+| commit_txn_step: forall t tid ver,
+      (trace_tid_last tid t = validate_read_item True 
+        /\ trace_no_writes tid t)
+      \/ (trace_tid_last tid t = complete_write_item ver
+			  /\ ~ trace_no_writes tid t)
+      -> sto_trace t
+      -> sto_trace ((tid, commit_txn (trace_commit_complete_last t)) :: t).
 
-| restart_txn_step: forall t tid,
+(*we don't need to rollback, once a transaction aborts, it will 'disappear'. A new transaction will do its work.*)
+(*| restart_txn_step: forall t tid newtid,
       trace_tid_last tid t = abort_txn (*we get abort and then restart*)
       -> sto_trace t
     (*our restart is to add back*)
-      -> sto_trace ((trace_filter_tid tid t) ++ t).
-(****************************************)
-(*Note!!!!!! *)
-(****************************************)
-    (*but !!! we need to change the tid for old ones*)
-    (*how to restart.......*)
+      -> sto_trace ((trace_rollback newtid (trace_commit_last t) (trace_filter_startreadwrite tid t)) ++ t).*)
 
-Example sto_trace_example_commit:  
-sto_trace [(2, commit_txn 1); (2, unlock_write_item 1); (2, complete_write_item 1); (2, validate_read_item True); (2, lock_write_item); (2, try_commit_txn); (2, write_item 4); (1, commit_txn 0); (1, validate_read_item True); (1, try_commit_txn); (1, read_item 0); (2, read_item 0);  (2, start_txn); (1, start_txn)].
+Example sto_trace_example_rollback:  
+sto_trace [(3, commit_txn 1); (3, validate_read_item True); (3, try_commit_txn); (3, read_item 1); (3, start_txn); (1, abort_txn); (1, validate_read_item False); (1, try_commit_txn); (2, commit_txn 1); (2, complete_write_item 1); (2, validate_read_item True); (2, lock_write_item); (2, try_commit_txn); (2, write_item 4); (1, read_item 0); (2, read_item 0);  (2, start_txn); (1, start_txn)].
 
-apply commit_write_txn_step.
-unfold trace_tid_last. simpl. auto.
-
-apply unlock_write_item_step.
-unfold trace_tid_last. simpl. split. auto.
-unfold trace_no_writes. simpl.
-intuition. 
-inversion H. inversion H3. inversion H7. inversion H11. inversion H15.
-simpl in *. auto.
-assert (trace_commit_last ([(2, validate_read_item True); (2, lock_write_item); (2, try_commit_txn); (2, write_item 4); (1, commit_txn 0); (1, validate_read_item True); (1, try_commit_txn); (1, read_item 0); (2, read_item 0); (2, start_txn); (1, start_txn)]) = 0).
-{ unfold trace_commit_last. simpl. auto. }
-assert (1 = S (trace_commit_last [(2, validate_read_item True); (2, lock_write_item); (2, try_commit_txn); (2, write_item 4); (1, commit_txn 0); (1, validate_read_item True); (1, try_commit_txn); (1, read_item 0);(2, read_item 0); (2, start_txn); (1, start_txn)])).
-{ rewrite H. auto. }
-rewrite H0.
-
-apply complete_write_item_step; rewrite <-H0.
-unfold trace_tid_last. simpl. split. auto.
-unfold trace_no_writes. simpl.
-intuition.
-inversion H1. inversion H5. inversion H9. inversion H13.
-simpl in *. auto.
-clear H H0.
-assert ((check_version (read_versions_tid 2 ([(2, lock_write_item); (2, try_commit_txn); (2, write_item 4); (1, commit_txn 0); (1, validate_read_item True); (1, try_commit_txn); (1, read_item 0); (2, read_item 0); (2, start_txn); (1, start_txn)])) (trace_commit_last ([(2, lock_write_item); (2, try_commit_txn); (2, write_item 4); (1, commit_txn 0); (1, validate_read_item True); (1, try_commit_txn); (1, read_item 0); (2, read_item 0); (2, start_txn); (1, start_txn)])) = True)).
-  {unfold check_version. simpl. auto. }
-  rewrite <- H.
-
-apply validate_read_item_step; rewrite H. 
-unfold trace_tid_last. simpl. right. auto. clear H.
-
-apply lock_write_item_step. split.
-unfold trace_tid_last. simpl. auto.
-unfold trace_no_writes. simpl.
-intuition.
-inversion H. inversion H3. simpl in *. auto.
-unfold check_lock_or_unlock. simpl. auto.
-
-apply try_commit_txn_step with (ver := 0) (val:= 4).
-unfold trace_tid_last. simpl. auto.
-
-apply write_item_step with (ver:=0) (oldval:=0).
-unfold trace_tid_last. simpl. right. left. auto.
-assert ((trace_commit_last ([(1, validate_read_item True); (1, try_commit_txn); (1, read_item 0); (2, read_item 0); (2, start_txn); (1, start_txn)])) = 0).
-{ unfold trace_commit_last. simpl. auto. }
+assert (trace_commit_complete_last [(3, validate_read_item True); (3, try_commit_txn); (3, read_item 1); (3, start_txn); (1, abort_txn); (1, validate_read_item False); (1, try_commit_txn); (2, commit_txn 1); (2, complete_write_item 1); (2, validate_read_item True); (2, lock_write_item); (2, try_commit_txn); (2, write_item 4); (1, read_item 0); (2, read_item 0); (2, start_txn); (1, start_txn)] = 1).
+{ unfold trace_commit_complete_last. simpl. auto. }
 rewrite <- H. 
-
-apply commit_readonly_txn_step; rewrite H. 
-unfold trace_tid_last. simpl. split. auto.
+apply commit_txn_step with (ver:= 0); rewrite H. 
+unfold trace_tid_last. simpl. left. split. auto.
 clear H.
 unfold trace_no_writes. simpl.
-repeat apply Forall_cons; simpl; auto.
-assert ((check_version (read_versions_tid 1 ([(1, try_commit_txn); (1, read_item 0); (2, read_item 0); (2, start_txn); (1, start_txn)])) (trace_commit_last ([(1, try_commit_txn); (1, read_item 0); (2, read_item 0); (2, start_txn); (1, start_txn)])) = True)).
+repeat apply Forall_cons; simpl; auto. clear H.
+assert ((check_version (read_versions_tid 3 ([(3, try_commit_txn); (3, read_item 1); (3, start_txn); (1, abort_txn); (1, validate_read_item False); (1, try_commit_txn); (2, commit_txn 1); (2, complete_write_item 1); (2, validate_read_item True); (2, lock_write_item); (2, try_commit_txn); (2, write_item 4); (1, read_item 0); (2, read_item 0); (2, start_txn); (1, start_txn)])) (trace_commit_last ([(3, try_commit_txn); (3, read_item 1); (3, start_txn); (1, abort_txn); (1, validate_read_item False); (1, try_commit_txn); (2, commit_txn 1); (2, complete_write_item 1); (2, validate_read_item True); (2, lock_write_item); (2, try_commit_txn); (2, write_item 4); (1, read_item 0); (2, read_item 0); (2, start_txn); (1, start_txn)])) = True)).
   {unfold check_version. simpl. auto. } 
-  rewrite <- H0.
+  rewrite <- H.
 
 apply validate_read_item_step.
 unfold trace_tid_last. simpl. left. split. auto.
 unfold trace_no_writes.
-repeat apply Forall_cons; simpl; auto.
-clear H H0.
+repeat apply Forall_cons; simpl; auto. rewrite H.
+clear H.
 
-apply try_commit_txn_step with (ver:= 0) (val:= 0).
+apply try_commit_txn_step with (ver:= 1) (val:= 0).
 unfold trace_tid_last. simpl. left. auto.
 
-assert (trace_commit_last [(2, read_item 0); (2, start_txn); (1, start_txn)] = 0).
+(*assert (trace_rollback 3 (trace_commit_last [(1, abort_txn); (1, validate_read_item False); (1, try_commit_txn); (2, commit_txn 1); (2, unlock_write_item 1); (2, complete_write_item 1); (2, validate_read_item True); (2, lock_write_item); (2, try_commit_txn); (2, write_item 4); (1, read_item 0); (2, read_item 0); (2, start_txn); (1, start_txn)]) (trace_filter_startreadwrite 1 [(1, abort_txn); (1, validate_read_item False); (1, try_commit_txn); (2, commit_txn 1); (2, unlock_write_item 1); (2, complete_write_item 1); (2, validate_read_item True); (2, lock_write_item); (2, try_commit_txn); (2, write_item 4); (1, read_item 0); (2, read_item 0); (2, start_txn); (1, start_txn)]) = [(3, read_item 1); (3, start_txn)]).
+unfold trace_rollback. simpl.
+unfold trace_commit_last. simpl. auto.
+
+assert ([(3, read_item 1); (3, start_txn); (1, abort_txn); (1, validate_read_item False); (1, try_commit_txn); (2, commit_txn 1); (2, unlock_write_item 1); (2, complete_write_item 1); (2, validate_read_item True); (2, lock_write_item); (2, try_commit_txn); (2, write_item 4); (1, read_item 0); (2, read_item 0); (2, start_txn); (1, start_txn)] = [(3, read_item 1); (3, start_txn)] ++ [(1, abort_txn); (1, validate_read_item False); (1, try_commit_txn); (2, commit_txn 1); (2, unlock_write_item 1); (2, complete_write_item 1); (2, validate_read_item True); (2, lock_write_item); (2, try_commit_txn); (2, write_item 4); (1, read_item 0); (2, read_item 0); (2, start_txn); (1, start_txn)]). auto.
+rewrite H0. rewrite <- H.
+apply restart_txn_step. unfold trace_tid_last. simpl. auto. clear H H0.
+*)
+
+assert (trace_commit_last [(3, start_txn); (1, abort_txn); (1, validate_read_item False); (1, try_commit_txn); (2, commit_txn 1); (2, complete_write_item 1); (2, validate_read_item True); (2, lock_write_item); (2, try_commit_txn); (2, write_item 4); (1, read_item 0); (2, read_item 0); (2, start_txn); (1, start_txn)] = 1).
 {unfold trace_commit_last; simpl. auto. }
 rewrite <- H.
-
-apply read_item_step with (val:=0) (oldver:=0); rewrite H. clear H.
+apply read_item_step with (val:=0) (oldver:=0); rewrite H.
 unfold trace_tid_last. simpl. left. auto.
-unfold check_lock_or_unlock. simpl. auto.
+unfold check_lock_or_unlock. simpl. auto. clear H.
+ 
+apply start_txn_step. 
+unfold trace_tid_last. simpl. auto.
 
-assert (trace_commit_last [(2, start_txn); (1, start_txn)] = 0).
-{unfold trace_commit_last; simpl. auto. }
-rewrite <- H0.
+apply abort_txn_step.
+unfold trace_tid_last. simpl. auto.
 
-apply read_item_step with (val:=0) (oldver:=0); rewrite H0. clear H H0.
-unfold trace_tid_last. simpl. left. auto.
-unfold check_lock_or_unlock. simpl. auto.
-
-apply start_txn_step. unfold trace_tid_last. auto.
-apply start_txn_step. unfold trace_tid_last. auto.
-
-apply empty_step.
-
-Example sto_trace_example_abort:  
-sto_trace [(1, abort_txn); (1, validate_read_item False); (1, try_commit_txn); (2, commit_txn 1); (2, unlock_write_item 1); (2, complete_write_item 1); (2, validate_read_item True); (2, lock_write_item); (2, try_commit_txn); (2, write_item 4); (1, read_item 0); (2, read_item 0);  (2, start_txn); (1, start_txn)].
-
-apply abort_readonly_txn_step.
-unfold trace_tid_last. simpl. split. auto.
-unfold trace_no_writes. simpl.
-repeat apply Forall_cons; simpl; auto.
-
-assert ((check_version (read_versions_tid 1 ([(1, try_commit_txn); (2, commit_txn 1); (2, unlock_write_item 1); (2, complete_write_item 1); (2, validate_read_item True); (2, lock_write_item); (2, try_commit_txn); (2, write_item 4); (1, read_item 0); (2, read_item 0); (2, start_txn); (1, start_txn)])) (trace_commit_last ([(1, try_commit_txn); (2, commit_txn 1); (2, unlock_write_item 1); (2, complete_write_item 1); (2, validate_read_item True); (2, lock_write_item); (2, try_commit_txn); (2, write_item 4); (1, read_item 0); (2, read_item 0); (2, start_txn); (1, start_txn)])) = False)).
+assert ((check_version (read_versions_tid 1 ([(1, try_commit_txn); (2, commit_txn 1); (2, complete_write_item 1); (2, validate_read_item True); (2, lock_write_item); (2, try_commit_txn); (2, write_item 4); (1, read_item 0); (2, read_item 0); (2, start_txn); (1, start_txn)])) (trace_commit_last ([(1, try_commit_txn); (2, commit_txn 1); (2, complete_write_item 1); (2, validate_read_item True); (2, lock_write_item); (2, try_commit_txn); (2, write_item 4); (1, read_item 0); (2, read_item 0); (2, start_txn); (1, start_txn)])) = False)).
 unfold check_version. simpl. auto.
 rewrite <- H. 
 apply validate_read_item_step. 
@@ -415,15 +420,24 @@ clear H.
 apply try_commit_txn_step with (ver:= 0) (val:= 4).
 unfold trace_tid_last. simpl. auto.
 
-apply commit_write_txn_step.
-unfold trace_tid_last. simpl. auto.
-
+assert (trace_commit_complete_last [(2, complete_write_item 1); (2, validate_read_item True); (2, lock_write_item); (2, try_commit_txn); (2, write_item 4); (1, read_item 0); (2, read_item 0); (2, start_txn); (1, start_txn)] = 1).
+{ unfold trace_commit_complete_last. simpl. auto. }
+rewrite <- H.
+apply commit_txn_step with (ver := 1); rewrite H.
+unfold trace_tid_last. simpl. right. split. auto.
+unfold trace_no_writes. simpl.
+intuition. 
+inversion H0. inversion H4. inversion H8. inversion H12. inversion H16.
+simpl in H19. auto. 
+(*
 apply unlock_write_item_step.
 unfold trace_tid_last. simpl. split. auto.
 unfold trace_no_writes. simpl.
 intuition. 
 inversion H. inversion H3. inversion H7. inversion H11. inversion H15.
 simpl in *. auto.
+*)
+clear H.
 assert (trace_commit_last ([(2, validate_read_item True); (2, lock_write_item); (2, try_commit_txn); (2, write_item 4); (1, read_item 0); (2, read_item 0); (2, start_txn); (1, start_txn)]) = 0).
 { unfold trace_commit_last. simpl. auto. }
 assert (1 = S (trace_commit_last [(2, validate_read_item True); (2, lock_write_item); (2, try_commit_txn); (2, write_item 4); (1, read_item 0); (2, read_item 0); (2, start_txn); (1, start_txn)])).
@@ -476,6 +490,94 @@ apply start_txn_step. unfold trace_tid_last. auto.
 
 apply empty_step.
 
+Example sto_trace_example_commit:  
+sto_trace [(2, commit_txn 1); (2, complete_write_item 1); (2, validate_read_item True); (2, lock_write_item); (2, try_commit_txn); (2, write_item 4); (1, commit_txn 0); (1, validate_read_item True); (1, try_commit_txn); (1, read_item 0); (2, read_item 0);  (2, start_txn); (1, start_txn)].
+
+assert (trace_commit_complete_last [(2, complete_write_item 1); (2, validate_read_item True); (2, lock_write_item); (2, try_commit_txn); (2, write_item 4); (1, commit_txn 0); (1, validate_read_item True); (1, try_commit_txn); (1, read_item 0); (2, read_item 0);  (2, start_txn); (1, start_txn)] = 1).
+{ unfold trace_commit_complete_last. simpl. auto. }
+rewrite <- H. 
+apply commit_txn_step with (ver := 1).
+unfold trace_tid_last; rewrite H. simpl. right. split. auto. clear H.
+unfold trace_no_writes. simpl.
+intuition. 
+inversion H. inversion H3. inversion H7. inversion H11. inversion H15.
+simpl in H18. auto. rewrite H. clear H.
+
+assert (trace_commit_last ([(2, validate_read_item True); (2, lock_write_item); (2, try_commit_txn); (2, write_item 4); (1, commit_txn 0); (1, validate_read_item True); (1, try_commit_txn); (1, read_item 0); (2, read_item 0); (2, start_txn); (1, start_txn)]) = 0).
+{ unfold trace_commit_last. simpl. auto. }
+assert (1 = S (trace_commit_last [(2, validate_read_item True); (2, lock_write_item); (2, try_commit_txn); (2, write_item 4); (1, commit_txn 0); (1, validate_read_item True); (1, try_commit_txn); (1, read_item 0);(2, read_item 0); (2, start_txn); (1, start_txn)])).
+{ rewrite H. auto. }
+rewrite H0.
+
+apply complete_write_item_step; rewrite <-H0.
+unfold trace_tid_last. simpl. split. auto.
+unfold trace_no_writes. simpl.
+intuition.
+inversion H1. inversion H5. inversion H9. inversion H13.
+simpl in *. auto.
+clear H H0.
+assert ((check_version (read_versions_tid 2 ([(2, lock_write_item); (2, try_commit_txn); (2, write_item 4); (1, commit_txn 0); (1, validate_read_item True); (1, try_commit_txn); (1, read_item 0); (2, read_item 0); (2, start_txn); (1, start_txn)])) (trace_commit_last ([(2, lock_write_item); (2, try_commit_txn); (2, write_item 4); (1, commit_txn 0); (1, validate_read_item True); (1, try_commit_txn); (1, read_item 0); (2, read_item 0); (2, start_txn); (1, start_txn)])) = True)).
+  {unfold check_version. simpl. auto. }
+  rewrite <- H.
+
+apply validate_read_item_step; rewrite H. 
+unfold trace_tid_last. simpl. right. auto. clear H.
+
+apply lock_write_item_step. split.
+unfold trace_tid_last. simpl. auto.
+unfold trace_no_writes. simpl.
+intuition.
+inversion H. inversion H3. simpl in *. auto.
+unfold check_lock_or_unlock. simpl. auto.
+
+apply try_commit_txn_step with (ver := 0) (val:= 4).
+unfold trace_tid_last. simpl. auto.
+
+apply write_item_step with (ver:=0) (oldval:=0).
+unfold trace_tid_last. simpl. right. left. auto.
+
+assert (trace_commit_complete_last [(1, validate_read_item True); (1, try_commit_txn); (1, read_item 0); (2, read_item 0); (2, start_txn); (1, start_txn)] = 0).
+{ unfold trace_commit_complete_last. simpl. auto. }
+rewrite <- H. 
+apply commit_txn_step with (ver:= 0); rewrite H. 
+unfold trace_tid_last. simpl. left. split. auto.
+clear H.
+unfold trace_no_writes. simpl.
+repeat apply Forall_cons; simpl; auto. clear H.
+
+assert ((check_version (read_versions_tid 1 ([(1, try_commit_txn); (1, read_item 0); (2, read_item 0); (2, start_txn); (1, start_txn)])) (trace_commit_last ([(1, try_commit_txn); (1, read_item 0); (2, read_item 0); (2, start_txn); (1, start_txn)])) = True)).
+  {unfold check_version. simpl. auto. } 
+  rewrite <- H.
+
+apply validate_read_item_step.
+unfold trace_tid_last. simpl. left. split. auto.
+unfold trace_no_writes.
+repeat apply Forall_cons; simpl; auto.
+clear H.
+
+apply try_commit_txn_step with (ver:= 0) (val:= 0).
+unfold trace_tid_last. simpl. left. auto.
+
+assert (trace_commit_last [(2, read_item 0); (2, start_txn); (1, start_txn)] = 0).
+{unfold trace_commit_last; simpl. auto. }
+rewrite <- H.
+
+apply read_item_step with (val:=0) (oldver:=0); rewrite H. clear H.
+unfold trace_tid_last. simpl. left. auto.
+unfold check_lock_or_unlock. simpl. auto.
+
+assert (trace_commit_last [(2, start_txn); (1, start_txn)] = 0).
+{unfold trace_commit_last; simpl. auto. }
+rewrite <- H0.
+
+apply read_item_step with (val:=0) (oldver:=0); rewrite H0. clear H H0.
+unfold trace_tid_last. simpl. left. auto.
+unfold check_lock_or_unlock. simpl. auto.
+
+apply start_txn_step. unfold trace_tid_last. auto.
+apply start_txn_step. unfold trace_tid_last. auto.
+
+apply empty_step.
 
 
 
